% Question 7

\begin{itemize}
    \item[(a)] If we denote the number of observations by $n$ and the number of 
    variables by $p$, then we let $x_{ij}$ denote the $i$th observation of the 
    $j$th variable. We calculate the Euclidian distances using the formula
    \begin{equation*}
        \begin{split}
            &d((X_1 = 0, X_2 = 0, X_3 = 0), (x_{i1}, x_{i2}, x_{i3})) \\
            = &\sqrt{{(0 - x_{i1})}^2 + {(0 - x_{i2})}^2 + {(0 - x_{i3})}^2} \\
            = &\sqrt{{(-x_{i1})}^2 + {(-x_{i2})}^2 + {(-x_{i3})}^2},
        \end{split}
    \end{equation*}
    for $i \in \lbrace 1, \dotsc, 6\rbrace$.\par
    Thus we have
    \begin{equation*}
        \begin{split}
            &d((X_1 = 0, X_2 = 0, X_3 = 0), (x_{11}, x_{12}, x_{13})) \\
            = &\sqrt{9^2} \\ 
            = &9,
        \end{split}
    \end{equation*}
    \begin{equation*}
        \begin{split}
            &d((X_1 = 0, X_2 = 0, X_3 = 0), (x_{21}, x_{22}, x_{23})) \\ 
            = &\sqrt{2^2} \\ 
            = &2,
        \end{split}
    \end{equation*}
    \begin{equation*}
        \begin{split}
            &d((X_1 = 0, X_2 = 0, X_3 = 0), (x_{31}, x_{32}, x_{33})) \\ 
            = &\sqrt{1^2 + 3^2} \\
            = &\sqrt{10} \\
            \approx &3.162278,
        \end{split}
    \end{equation*}
    \begin{equation*}
        \begin{split}
            &d((X_1 = 0, X_2 = 0, X_3 = 0), (x_{41}, x_{42}, x_{43})) \\
            = &\sqrt{1^2 + 2^2} \\ 
            = &\sqrt{5} \\ 
            \approx &2.236068,
        \end{split}
    \end{equation*}
    \begin{equation*}
        \begin{split}
            &d((X_1 = 0, X_2 = 0, X_3 = 0), (x_{51}, x_{52}, x_{53})) \\ 
            = &\sqrt{(-1)^2 + 1^2} \\
            = &\sqrt{2} \\ 
            \approx &1.414214,
        \end{split}
    \end{equation*}
    and 
    \begin{equation*}
        \begin{split}
            &d((X_1 = 0, X_2 = 0, X_3 = 0), (x_{61}, x_{62}, x_{63})) \\ 
            = &\sqrt{1^2 + 1^2 + 1^2} \\
            = &\sqrt{3} \\ 
            \approx &1.732051.
        \end{split}
    \end{equation*}
    \item[(b)]
    \item[(c)]
    \item[(d)]
\end{itemize}
