% Exercise 3.12

\begin{itemize}
    \item[(a)] The coefficient estimate for the regression of $X$ onto $Y$ is the same
        as the coefficient estimate for the regression of $Y$ onto $X$ in the case where 
        \[
            \sum_{i' = 1}^n x_{i'}^2 = \sum_{i' = 1}^n y_{i'}^2,
        \]
        for $x_{i'}$ and $y_{i'}$ in the expression
        \[
            \hat{\beta} = \Biggl(\sum_{i = 1}^n x_i y_i \Biggr) / 
            \Biggl(\sum_{i' = 1}^n x_{i'}^2 \Biggr).
        \]
    \item[(b)] 
\end{itemize}
