% Exercise 3.5

\begin{proof}
    We have
    \begin{equation*}
        \begin{split}
            \hat{y}_i &= x_i \hat{\beta} \\
                      &= \frac{x_i \sum_{i'=1}^{n} x_{i'} y_{i'}}{\sum_{i'=1}^{n} 
                          x_{i'}^{2}} \\
                      &= \sum_{i'=1}^n \Biggl(\frac{x_i x_{i'} y_{i'}}
                          {\sum_{i'=1}^{n} x_{i'}^{2}} \Biggr) \\
                      &= \sum_{i'=1}^n \Biggl(\frac{x_i x_{i'}}
                          {\sum_{i'=1}^{n} x_{i'}^{2}} y_{i'}\Biggr) \\
                      &= \sum_{i'=1}^n a_{i'} y_{i'},
        \end{split}
    \end{equation*}
    where
    \[
        a_{i'} = \frac{x_i x_{i'}}{\sum_{i'=1}^{n} x_{i'}^{2}},
    \]
    for fixed $i$ and variable $i'$.
\end{proof}
