% Exercise 3.7

\begin{proof}
    If we assume $\bar{x} = \bar{y} = 0$, then the simple linear regression of
    $Y$ onto $X$ is given by
    \[
        \hat{y} = \hat{\beta}_0 + \hat{\beta}_1 x.
    \]
    Now we have
    \begin{equation*}
        \begin{split}
            R^2 &= \frac{\text{TSS} - \text{RSS}}{\text{TSS}} \\
                &= \frac{\sum_{i=1}^{n}{(y_i - \bar{y})}^{2} 
                    - \sum_{i=1}^{n}{(y_i - \hat{y_i})}^{2}}
                    {\sum_{i=1}^{n}{(y_i - \bar{y})}^{2}} \\
                &= \frac{\sum_{i=1}^{n}[{(y_i - \bar{y})}^{2} 
                    - {(y_i - \hat{y_i})}^{2}]}
                    {\sum_{i=1}^{n}{(y_i - \bar{y})}^{2}} \\
                &= \frac{\sum_{i=1}^{n}[{(y_i - \bar{y})}^{2} 
                    - {(y_i - \hat{\beta}_0 - \hat{\beta}_1 x_i)}^{2}}
                    {\sum_{i=1}^{n}{(y_i - \bar{y})}^{2}} \\
                &= \frac{\sum_{i=1}^{n}[{(y_i - \bar{y})}^{2} 
                    - {(y_i - \bar{y} + \hat{\beta}_1 \bar{x} 
                    - \hat{\beta}_1 x_i)}^{2}]}
                    {\sum_{i=1}^{n}{(y_i - \bar{y})}^{2}} \\
                &= \frac{\sum_{i=1}^{n}[{(y_i - \bar{y})}^{2} 
                    - {(y_i - \bar{y} + \hat{\beta}_1 [\bar{x} - x_i])}^{2}]}
                    {\sum_{i=1}^{n}{(y_i - \bar{y})}^{2}}.
        \end{split}
    \end{equation*}
    Then, 
    \begin{equation*}
        \begin{split}
            \qquad &{(y_i - \bar{y} + \hat{\beta}_1 [\bar{x} - x_i])}^{2} \\
            = &\, y_i^2 - 2y_i\bar{y} + 2y_i\hat{\beta}_1(\bar{x} - x_i)
                - \bar{y}^2 - \bar{y}\hat{\beta}_1(\bar{x} - x_i) + \hat{\beta}_1^2
                {(\bar{x} - x_i)}^{2} \\
            = &\, {(y_i - \bar{y})}^{2} - 2\bar{y}^2 + \hat{\beta}_1(\bar{x} - x_i)
                (2y_i - \bar{y}) + \hat{\beta}_1^2{(\bar{x} - x_i)}^{2},
        \end{split}
    \end{equation*}
    so that
    \begin{equation*}
        \begin{split}
            R^2 &= \frac{\text{TSS} - \text{RSS}}{\text{TSS}} \\
                &= \frac{\sum_{i=1}^{n}[-2\bar{y}^2 + \hat{\beta}_1(\bar{x} - x_i)
                (2y_i - \bar{y}) + \hat{\beta}_1^2{(\bar{x} - x_i)}^{2}]}
                    {\sum_{i=1}^{n}{(y_i - \bar{y})}^{2}}.
        \end{split}
    \end{equation*}
\end{proof}
